verif/trie/tactics.v
@@ -1,6 +1,63 @@
 (** * tactics.v : General Tactics *)
 Require Import VST.floyd.proofauto.
 
+Tactic Notation "if_tac" := 
+  match goal with |- context [if ?a then _ else _] =>
+    lazymatch type of a with
+    | sumbool _ _ => destruct a as [?H | ?H]
+    | option _ => destruct a eqn:?H
+    | bool => fail "Use simple_if_tac instead of if_tac, since your expression"a" has type bool"
+    | ?t => fail "Use if_tac only for sumbool; your expression"a" has type" t
+   end end.
+
+Tactic Notation "if_tac" simple_intropattern(H)
+   := match goal with |- context [if ?a then _ else _] =>
+    lazymatch type of a with
+    | sumbool _ _ => destruct a as H
+    | option _ => destruct a eqn:H
+    | bool => fail "Use simple_if_tac instead of if_tac, since your expression"a" has type bool"
+    | ?t => fail "Use if_tac only for sumbool; your expression"a" has type" t
+   end end.
+
+Tactic Notation "if_tac" "in" hyp(H0)
+ := match type of H0 with context [if ?a then _ else _] =>
+    lazymatch type of a with
+    | sumbool _ _ => destruct a as [?H | ?H]
+    | option _ => destruct a eqn:?H
+    | bool => fail "Use simple_if_tac instead of if_tac, since your expression"a" has type bool"
+    | ?t => fail "Use if_tac only for sumbool; your expression"a" has type" t
+   end end.
+
+Tactic Notation "if_tac" simple_intropattern(H) "in" hyp(H1)
+ := match type of H1 with context [if ?a then _ else _] => 
+    lazymatch type of a with
+    | sumbool _ _ => destruct a as H
+    | option _ => destruct a eqn:H
+    | bool => fail "Use simple_if_tac instead of if_tac, since your expression"a" has type bool"
+    | ?t => fail "Use if_tac only for sumbool; your expression"a" has type" t
+   end end.
+
+Tactic Notation "match_tac" := 
+  match goal with |- context [match ?a with _ => _ end] =>
+                  destruct a eqn:?H
+  end.
+
+Tactic Notation "match_tac" simple_intropattern(H) :=
+  match goal with |- context [match ?a with _ => _ end] =>
+                      destruct a eqn:H
+  end.
+
+Tactic Notation "match_tac" "in" hyp(H0) :=
+  match type of H0 with context [match ?a with _ => _ end] =>
+                        destruct a eqn:?H
+  end.
+
+Tactic Notation "match_tac" simple_intropattern(H) "in" hyp(H1) :=
+  match type of H1 with context [match ?a with _ => _ end] =>
+                        destruct a eqn:H
+  end.
+
+
 Ltac elim_cast_pointer' term t :=
   match t with
   | force_val (sem_cast_pointer ?t') => elim_cast_pointer' term t'
